LocalHints.v
@@ -1,0 +1,103 @@
+(* NOTE(dbp 2017-03-26): Often when inverting, we only want to handle
+   cases that are _not_ variables. This will fail if C is a variable
+   of type T *)
+Ltac not_var C T :=
+  match goal with
+  |[ C' : T |- _ ] =>
+   match C with
+   | C' => fail 2
+   | _ => fail 1
+   end
+  | _ => idtac
+  end.
+
+Tactic Notation "hint" constr(E) :=
+  let H := fresh "Hint" in
+  let t := type of E in
+  assert (H : t) by exact E.
+
+Tactic Notation "hint" constr(E) "," constr(E1) := hint E; hint E1.
+Tactic Notation "hint" constr(E) "," constr(E1) "," constr(E2) :=
+  hint E; hint E1; hint E2.
+Tactic Notation "hint" constr(E) "," constr(E1) "," constr(E2) "," constr(E3) :=
+  hint E; hint E1; hint E2; hint E3.
+Tactic Notation "hint" constr(E) "," constr(E1) "," constr(E2) "," constr(E3) "," constr(E4) :=
+  hint E; hint E1; hint E2; hint E3; hint E4.
+Tactic Notation "hint" constr(E) "," constr(E1) "," constr(E2) "," constr(E3) "," constr(E4) "," constr(E5) :=
+  hint E; hint E1; hint E2; hint E3; hint E4; hint E5.
+
+
+Inductive RR (A : Prop) : Prop :=
+| rewrite_rule : forall a : A, RR A.
+
+Definition unRR (A : Prop) (r : RR A) :=
+  match r with
+  | rewrite_rule rr => rr
+  end.
+
+Tactic Notation "hint_rewrite" constr(E) := 
+  let H := fresh "Hint" in
+  let t := type of E in
+  assert (H : RR t) by exact (rewrite_rule E).
+
+Tactic Notation "hint_rewrite" constr(E) "," constr(E1) :=
+  hint_rewrite E; hint_rewrite E1.
+Tactic Notation "hint_rewrite" constr(E) "," constr(E1) "," constr(E2) :=
+  hint_rewrite E; hint_rewrite E1; hint_rewrite E2.
+Tactic Notation "hint_rewrite" constr(E) "," constr(E1) "," constr(E2) "," constr(E3) :=
+  hint_rewrite E; hint_rewrite E1; hint_rewrite E2; hint_rewrite E3.
+
+Ltac swap_rewrite t :=
+  match type of t with
+  | ?v1 = ?v2 => constr:(eq_sym t) 
+  | forall x : ?T, _ =>
+    (* let ret :=  *)constr:(fun x : T => let r := t x in 
+                                      ltac:(let r' := swap_rewrite r in
+                                            exact r')) (* in *)
+    (* let ret' := (eval cbv zeta in ret) in *)
+    (* constr:(ret) *)
+  end.
+
+Tactic Notation "hint_rewrite" "<-" constr(E) := 
+  let H := fresh "Hint" in
+  let E' := swap_rewrite E in
+  let t := type of E' in
+  assert (H : RR t) by exact (rewrite_rule E').
+
+
+Hint Extern 5 => match goal with
+                |[H : RR (_ = _) |- _] =>
+                 progress (rewrite (unRR H) in *)
+                end.
+Hint Extern 5 => match goal with
+                |[H : RR (forall _, _ = _) |- _] =>
+                 progress (rewrite (unRR H) in *)
+                end.
+Hint Extern 5 => match goal with
+                |[H : RR (forall _ _, _ = _) |- _] =>
+                 progress (rewrite (unRR H) in *)
+                end.
+Hint Extern 5 => match goal with
+                |[H : RR (forall _ _ _, _ = _) |- _] =>
+                 progress (rewrite (unRR H) in *)
+                end.
+Hint Extern 5 => match goal with
+                |[H : RR (forall _ _ _ _, _ = _) |- _] =>
+                 progress (rewrite (unRR H) in *) 
+                end.
+Hint Extern 5 => match goal with
+                |[H : RR (forall _ _ _ _ _, _ = _) |- _] =>
+                 progress (rewrite (unRR H) in *) 
+                end.
+Hint Extern 5 => match goal with
+                |[H : RR (forall _ _ _ _ _ _, _ = _) |- _] =>
+                 progress (rewrite (unRR H) in *) 
+                end.
+Hint Extern 5 => match goal with
+                |[H : RR (forall _ _ _ _ _ _ _, _ = _) |- _] =>
+                 progress (rewrite (unRR H) in *) 
+                end.
+
+Tactic Notation "hint_tactic" constr(name) :=
+  let H := fresh "HintEnable" in
+  assert (H : name = True) by reflexivity.
